WIP typeclass to the rescue
or to the hell, i am not sure yet

minuska/theories/notations.v
@@ -7,16 +7,14 @@ From Minuska Require Import
     flattened
 .
 
-
-Declare Scope RuleLhsScope.
-Declare Scope ExprScope.
-Declare Scope RuleScsScope.
+Declare Scope SymbolicScope.
 Declare Scope ConcreteScope.
+(*Declare Scope RuleScsScope.*)
 
-Delimit Scope RuleLhsScope with rule_lhs.
-Delimit Scope ExprScope with expr.
-Delimit Scope RuleScsScope with rule_scs.
+Delimit Scope SymbolicScope with symbolic.
 Delimit Scope ConcreteScope with concrete.
+(*Delimit Scope RuleScsScope with rule_scs.*)
+
 
 Record ExprAndBoV {Σ : StaticModel} : Type := mkExprAndBoV {
     eab_expr : Expression ;
@@ -25,60 +23,127 @@ Record ExprAndBoV {Σ : StaticModel} : Type := mkExprAndBoV {
 
 Arguments mkExprAndBoV {Σ} eab_expr eab_bov.
 
+Class TagLHS := mkTagLHS {}.
+Class TagRHS := mkTagRHS {}.
+
+Class Resolver {Σ : StaticModel} := {
+    operand_type : Type ;
+    (*operand_of_eab : ExprAndBoV -> operand_type ; *)
+    inject_variable : variable -> operand_type ;
+}.
+
+#[export]
+Instance Resolver_1 {Σ : StaticModel} {_T1 : TagLHS} : Resolver := {
+    operand_type := BuiltinOrVar ;
+    (*operand_of_eab := eab_bov ;*)
+    inject_variable := bov_variable;
+}.
+
+#[export]
+Instance Resolver_2 {Σ : StaticModel} {_T2 : TagRHS} : Resolver := {
+    operand_type := Expression ;
+    (*operand_of_eab := eab_expr ;*)
+    inject_variable := ft_variable;
+}.
+
+Class Coercer {Σ : StaticModel} (T : Type) := {
+    mycoerc : T -> Expression ;
+}.
+
+#[export]
+Instance Coercer_eab {Σ : StaticModel} {_T : TagRHS} : Coercer ExprAndBoV := {|
+    mycoerc := eab_expr ;
+|}.
+
+#[export]
+Instance Coercer_expr {Σ : StaticModel} {_T : TagRHS} : Coercer Expression := {|
+    mycoerc := fun x => x ;
+|}.
+
 (*
-(* #[reversible] *)
-Coercion eab_expr : ExprAndBoV >-> Expression.
-(* #[reversible] *)
-Coercion eab_bov : ExprAndBoV >-> BuiltinOrVar.
-*)
 Notation "'$' x" :=
     (mkExprAndBoV (ft_variable x) (bov_variable x))
     (at level 40)
 .
+*)
 
-Structure MyApplyLhs {Σ : StaticModel} := {
-    mal_T2 : Type ;
-    my_apply_lhs :
-        AppliedOperator' symbol BuiltinOrVar ->
+Notation "'$' x" :=
+    (inject_variable x)
+    (at level 40)
+.
+
+Class MyApply
+    {Σ : StaticModel}
+    {_R : Resolver}
+    (T2 : Type)
+:= {
+    my_apply : 
+        AppliedOperator' symbol operand_type ->
+        T2 ->
+        AppliedOperator' symbol operand_type ;
+}.
+
+#[export]
+Instance MyApply_direct_operand
+    {Σ : StaticModel}
+    {_R : Resolver}
+    : MyApply operand_type
+:= {|
+    my_apply := fun x y => ao_app_operand x y ;
+|}.
+
+(*
+#[export]
+Instance MyApply_eab_operand
+    {Σ : StaticModel}
+    {_R : Resolver}
+    : MyApply ExprAndBoV
+:= {|
+    my_apply := fun x y => ao_app_operand x (operand_of_eab y) ;
+|}.
+*)
+#[export]
+Instance MyApply_ao
+    {Σ : StaticModel}
+    {_R : Resolver}
+    : MyApply (AppliedOperator' symbol operand_type)
+:= {|
+    my_apply := fun x y => @ao_app_ao symbol _ x y ;
+|}.
+
+
+(*
+
+Structure MyApply {Σ : StaticModel} {_R : Resolver} := {
+    #[canonical=yes] mal_T2 : Type ;
+    #[canonical=no] my_apply :
+        AppliedOperator' symbol operand_type ->
         mal_T2 ->
-        AppliedOperator' symbol BuiltinOrVar ;
+        AppliedOperator' symbol operand_type ;
 }.
 
-Arguments my_apply_lhs {_} {m} _ _.
-Arguments my_apply_lhs : simpl never.
+Arguments my_apply {_} {_} {m} _ _.
+Arguments my_apply : simpl never.
 
-Definition MyApplyLhs_operand {Σ : StaticModel} : MyApplyLhs := {|
-    my_apply_lhs := fun x y => ao_app_operand x (eab_bov y) ;
+Definition MyApply_operand
+    {Σ : StaticModel}
+    {_R : Resolver}
+    : MyApply
+:= {|
+    my_apply := fun x y => ao_app_operand x y ;
 |}.
-Canonical MyApplyLhs_operand.
+Canonical MyApply_operand.
 
-Definition MyApplyLhs_ao {Σ : StaticModel} : MyApplyLhs := {|
-    my_apply_lhs := fun x y => @ao_app_ao symbol BuiltinOrVar x y ;
+Definition MyApply_ao
+    {Σ : StaticModel}
+    {_R : Resolver}
+    : MyApply
+:= {|
+    my_apply := fun x y => @ao_app_ao symbol _ x y ;
 |}.
-Canonical MyApplyLhs_ao.
-
-Structure MyApplyRhs {Σ : StaticModel} := {
-    mar_T2 : Type ;
-    my_apply_rhs :
-        AppliedOperator' symbol Expression ->
-        mar_T2 ->
-        AppliedOperator' symbol Expression ;
-}.
-
-Arguments my_apply_rhs {_} {m} _ _.
-Arguments my_apply_rhs : simpl never.
-
-Definition MyApplyRhs_operand {Σ : StaticModel} : MyApplyRhs := {|
-    my_apply_rhs := fun x y => ao_app_operand x (eab_expr y) ;
-|}.
-Canonical MyApplyRhs_operand.
-
-Definition MyApplyRhs_ao {Σ : StaticModel} : MyApplyRhs := {|
-    my_apply_rhs := fun x y => @ao_app_ao symbol Expression x y ;
-|}.
-Canonical MyApplyRhs_ao.
-
-
+Canonical MyApply_ao.
+Print Canonical Projections.
+*)
 Structure MyApplyConcrete {Σ : StaticModel} := {
     mac_T2 : Type ;
     my_apply_c :
@@ -104,16 +169,13 @@ Notation "f [<>]" := (ao_operator f)
     (at level 90)
 .
 
-Notation "f [< y , .. , z >]"
-    := (my_apply_lhs .. (my_apply_lhs (ao_operator f) y) .. z)
-    (at level 90)
-    : RuleLhsScope
-.
+Check @my_apply.
+
+Definition my_type_of {T : Type} (x : T) : Type := T.
 
 Notation "f [< y , .. , z >]"
-    := (my_apply_rhs .. (my_apply_rhs (ao_operator f) y) .. z)
+    := (@my_apply _ _ (my_type_of z) _ .. (@my_apply _ _ (my_type_of y) _ (ao_operator f) y) .. z)
     (at level 90)
-    : ExprScope
 .
 
 Notation "f [< y , .. , z >]"
@@ -122,12 +184,14 @@ Notation "f [< y , .. , z >]"
     : ConcreteScope
 .
 
+About mkFlattenedRewritingRule.
+
 Notation "'llrule' l => r 'requires' s"
     := (@mkFlattenedRewritingRule
         _
-        (l)%rule_lhs
-        (r)%expr
-        (s)%rule_scs
+        ((fun (_:TagLHS) => l) mkTagLHS)
+        ((fun (_:TagRHS) => r) mkTagRHS)%symbolic
+        (s)%symbolic
     )
     (at level 200)
 .
